fmap_functions.thy
@@ -1,0 +1,14 @@
+theory fmap_functions
+  imports Main
+    "~~/src/HOL/Library/Finite_Map"
+begin
+
+abbreviation lookupsyntax ("_ .[_]"[25,25]25) where
+"m.[x] \<equiv> fmlookup m x"
+
+abbreviation lookupsyntax2 ("_ ![_]"[25,25]25) where
+"m![x] \<equiv> the (fmlookup m x)"
+
+
+
+end
